proof/Anomaly.thy
@@ -15,21 +15,48 @@ definition has_g1a :: "history \<Rightarrow> bool" where
                                   (AWrite k v1 a v2 r) \<in> (all_aops t1) \<and>
                                   (ARead k v2) \<in> (all_aops t2))"
 
-text \<open>An empty history does not have an aborted read.\<close>
+text \<open>An empty history does not have an aborted read. We use key variables since key is opaque.\<close>
 
-lemma "\<not>(has_g1a (History {(register 1)} {} {(KeyVersionOrder 1 [[0]])}))"
+lemma "\<not>(has_g1a (History {(register k)} {} {(KeyVersionOrder k [[0]])}))"
   by (simp add:has_g1a_def)
 
 text "But this history does: we write 1 and fail to commit, then read it! We don't actually
 have to constrain the version order for this to happen, either."
 
-lemma "has_g1a (History {(register 1)}
-                        {(ATxn [(AWrite 1 [0] 1 [1] [])] False),
-                         (ATxn [(ARead 1 [1])] True)}
+lemma "has_g1a (History {(register k)}
+                        {(ATxn [(AWrite k [0] 1 [1] [])] False),
+                         (ATxn [(ARead k [1])] True)}
                         kvo)"
   using has_g1a_def by fastforce
 
-(* TODO: intermediate read, dirty update *)
+text \<open>An intermediate read, or G1b, implies a committed transaction t2 reads a version v2 of key k
+that was produced by a non-final write of another committed transaction t1. A write is non-final
+(intermediate) if there exists a later write to the same key in the same transaction.\<close>
+
+definition is_intermediate_awrite :: "aop list \<Rightarrow> key \<Rightarrow> aop \<Rightarrow> bool" where
+"is_intermediate_awrite ops k w \<equiv>
+  (\<exists>i j. i < length ops \<and> j < length ops \<and> i < j \<and>
+         ops ! i = w \<and> op_type (ops ! j) = Write \<and> key (ops ! j) = k)"
+
+definition has_g1b :: "history \<Rightarrow> bool" where
+"has_g1b h \<equiv> (\<exists>t1 t2 k v1 a v2 r. (t1 \<in> (all_atxns h)) \<and>
+                                  (t2 \<in> (all_atxns h)) \<and>
+                                  (a_is_committed t1) \<and>
+                                  (a_is_committed t2) \<and>
+                                  (AWrite k v1 a v2 r) \<in> set (a_ops t1) \<and>
+                                  is_intermediate_awrite (a_ops t1) k (AWrite k v1 a v2 r) \<and>
+                                  (ARead k v2) \<in> (all_aops t2))"
+
+text \<open>A dirty update occurs when a committed transaction T2 contains a write which acts on a
+version produced by an uncommitted (aborted) transaction T1. Information from the aborted
+transaction leaks into the committed state via writes rather than reads.\<close>
+
+definition has_dirty_update :: "history \<Rightarrow> bool" where
+"has_dirty_update h \<equiv> (\<exists>t1 t2 k v1 a1 vi r1 a2 v2 r2.
+  (t1 \<in> (all_atxns h)) \<and> (t2 \<in> (all_atxns h)) \<and>
+  (\<not>(a_is_committed t1)) \<and> (a_is_committed t2) \<and>
+  (AWrite k v1 a1 vi r1) \<in> (all_aops t1) \<and>
+  (AWrite k vi a2 v2 r2) \<in> (all_aops t2))"
 
 section \<open>Cyclic Anomalies\<close>
 
@@ -40,6 +67,11 @@ definition has_g0 :: "history \<Rightarrow> bool" where
 
 text \<open>For example...\<close>
 
+text \<open>We show ww-depends by providing explicit write witnesses and unfolding the definitions.
+The key steps: (1) each write is in ext_awrites because it's the last write to its key in the
+transaction, (2) they share the same key x, and (3) v1 immediately precedes v2 in the version
+order for x.\<close>
+
 lemma ww_depends_ex:
   assumes "(distinct [x,y]) \<and> (distinct [v0,v1,v2])"
   shows "ww_depends (History objs
@@ -49,23 +81,100 @@ lemma ww_depends_ex:
                           (KeyVersionOrder y [v0,v1,v2])})
                       (ATxn [(AWrite x v0 a1 v1 r1), (AWrite y v1 a2 v2 r2)] True)
                       (ATxn [(AWrite y v0 a1 v1 r1), (AWrite x v1 a2 v2 r2)] True)"
-  apply (simp add:ww_depends_def)
-proof-
-  obtain t1 t2 where "t1 = (ATxn [(AWrite x v0 a1 v1 r1), (AWrite y v1 a2 v2 r2)] True) \<and>
-                      t2 = (ATxn [(AWrite y v0 a1 v1 r1), (AWrite x v1 a2 v2 r2)] True)"
-    by blast
-  oops
+proof -
+  have xy: "x \<noteq> y" and dv: "v0 \<noteq> v1" "v0 \<noteq> v2" "v1 \<noteq> v2" using assms by auto
+  let ?t1 = "ATxn [(AWrite x v0 a1 v1 r1), (AWrite y v1 a2 v2 r2)] True"
+  let ?t2 = "ATxn [(AWrite y v0 a1 v1 r1), (AWrite x v1 a2 v2 r2)] True"
+  let ?h = "History objs {?t1, ?t2}
+              {(KeyVersionOrder x [v0,v1,v2]), (KeyVersionOrder y [v0,v1,v2])}"
+  let ?w1 = "AWrite x v0 a1 v1 r1"
+  let ?w2 = "AWrite x v1 a2 v2 r2"
+  have w1_in: "?w1 \<in> ext_awrites ?t1" using xy by (auto simp: ran_def)
+  have w2_in: "?w2 \<in> ext_awrites ?t2" using xy by (auto simp: ran_def)
+  have next_h: "is_next_in_history ?h x v1 v2"
+    unfolding is_next_in_history_def
+    apply simp
+    apply (rule_tac x="KeyVersionOrder x [v0, v1, v2]" in exI)
+    using dv by auto
+  show ?thesis
+    unfolding ww_depends_def
+    apply (rule_tac x="?w1" in exI)
+    apply (rule_tac x="?w2" in exI)
+    using w1_in w2_in next_h by simp
+qed
 
+text \<open>The has_g0 example requires constructing a full cycle in the DSG. This involves
+two ww-dependency edges (one per key) forming a cycle between the two transactions.\<close>
 
-lemma
+text \<open>We also need the reverse direction: t2 ww-depends on t1 via key y.\<close>
+
+lemma ww_depends_ex_rev:
+  assumes "(distinct [x,y]) \<and> (distinct [v0,v1,v2])"
+  shows "ww_depends (History objs
+                         {(ATxn [(AWrite x v0 a1 v1 r1), (AWrite y v1 a2 v2 r2)] True),
+                          (ATxn [(AWrite y v0 a1 v1 r1), (AWrite x v1 a2 v2 r2)] True)}
+                         {(KeyVersionOrder x [v0,v1,v2]),
+                          (KeyVersionOrder y [v0,v1,v2])})
+                      (ATxn [(AWrite y v0 a1 v1 r1), (AWrite x v1 a2 v2 r2)] True)
+                      (ATxn [(AWrite x v0 a1 v1 r1), (AWrite y v1 a2 v2 r2)] True)"
+proof -
+  have xy: "x \<noteq> y" and dv: "v0 \<noteq> v1" "v0 \<noteq> v2" "v1 \<noteq> v2" using assms by auto
+  let ?t1 = "ATxn [(AWrite x v0 a1 v1 r1), (AWrite y v1 a2 v2 r2)] True"
+  let ?t2 = "ATxn [(AWrite y v0 a1 v1 r1), (AWrite x v1 a2 v2 r2)] True"
+  let ?h = "History objs {?t1, ?t2}
+              {(KeyVersionOrder x [v0,v1,v2]), (KeyVersionOrder y [v0,v1,v2])}"
+  have w1_in: "AWrite y v0 a1 v1 r1 \<in> ext_awrites ?t2" using xy by (auto simp: ran_def)
+  have w2_in: "AWrite y v1 a2 v2 r2 \<in> ext_awrites ?t1" using xy by (auto simp: ran_def)
+  have next_h: "is_next_in_history ?h y v1 v2"
+    unfolding is_next_in_history_def
+    apply simp
+    apply (rule_tac x="KeyVersionOrder y [v0, v1, v2]" in exI)
+    using dv by auto
+  show ?thesis
+    unfolding ww_depends_def
+    apply (rule_tac x="AWrite y v0 a1 v1 r1" in exI)
+    apply (rule_tac x="AWrite y v1 a2 v2 r2" in exI)
+    using w1_in w2_in next_h by simp
+qed
+
+text \<open>Now we construct the cycle. The DSG uses tail=adep_tail (third component) and
+head=adep_head (first component). For ADep t1 WW t2, tail=t2 and head=t1.
+So the cycle path [ADep t2 WW t1, ADep t1 WW t2] starts at tail(e1)=t1,
+goes to head(e1)=t2, then tail(e2)=t2 matches, and head(e2)=t1 completes the cycle.\<close>
+
+lemma has_g0_ex:
   assumes "(distinct [x,y]) \<and> (distinct [v0,v1,v2])"
   shows "has_g0 (History objs
                          {(ATxn [(AWrite x v0 a1 v1 r1), (AWrite y v1 a2 v2 r2)] True),
                           (ATxn [(AWrite y v0 a1 v1 r1), (AWrite x v1 a2 v2 r2)] True)}
                          {(KeyVersionOrder x [v0,v1,v2]),
                           (KeyVersionOrder y [v0,v1,v2])})"
-  apply (simp add:has_g0_def dsg_def path_def cycle_def)
-  oops
+proof -
+  have xy: "x \<noteq> y" using assms by auto
+  let ?t1 = "ATxn [(AWrite x v0 a1 v1 r1), (AWrite y v1 a2 v2 r2)] True"
+  let ?t2 = "ATxn [(AWrite y v0 a1 v1 r1), (AWrite x v1 a2 v2 r2)] True"
+  let ?h = "History objs {?t1, ?t2}
+              {(KeyVersionOrder x [v0,v1,v2]), (KeyVersionOrder y [v0,v1,v2])}"
+  let ?G = "dsg ?h"
+  have ww12: "ww_depends ?h ?t1 ?t2" using ww_depends_ex assms by blast
+  have ww21: "ww_depends ?h ?t2 ?t1" using ww_depends_ex_rev assms by blast
+  let ?e1 = "ADep ?t2 WW ?t1"
+  let ?e2 = "ADep ?t1 WW ?t2"
+  let ?p = "[?e1, ?e2]"
+  have e1_in: "?e1 \<in> arcs ?G" using ww21 by (auto simp: dsg_def)
+  have e2_in: "?e2 \<in> arcs ?G" using ww12 by (auto simp: dsg_def)
+  have t1_vert: "?t1 \<in> verts ?G" by (simp add: dsg_def)
+  have t1_ne_t2: "?t1 \<noteq> ?t2" using xy by auto
+  have cas_ok: "cas ?G ?t1 ?p ?t1" by (simp add: dsg_def)
+  have path_ok: "path ?G ?t1 ?p ?t1"
+    unfolding path_def using t1_vert e1_in e2_in cas_ok by auto
+  have dist_ok: "distinct (tl (path_verts ?G ?t1 ?p))"
+    using t1_ne_t2 by (simp add: dsg_def)
+  have "cycle ?G ?p"
+    unfolding cycle_def using path_ok dist_ok by auto
+  moreover have "path_dep_types ?p = {WW}" by simp
+  ultimately show ?thesis unfolding has_g0_def by blast
+qed
 
 text \<open>A G1c anomaly is a cycle comprised of write-write and write-read dependencies. We diverge from
 Adya here in classifying G0 and G1c as distinct classes; feels more useful to distinguish them.\<close>
